Refactor to use ZFC_in_HOL

Locally_Nameless_Lambda_Calculus/LN_Lambda_Semantics.thy
@@ -1,234 +1,9 @@
 theory LN_Lambda_Semantics
-  imports LN_Lambda_Typing
+  imports
+    LN_Lambda_Typing
+    "HOL-Library.FuncSet"
+    ZFC_in_HOL.ZFC_Typeclasses
 begin
-
-term monoid
-
-class domain_universe =
-  fixes \<U> :: "'a set set" and ap_domain :: "'a \<Rightarrow> 'a \<Rightarrow> 'a"
-  assumes no_empty_domain: "{} \<notin> \<U>"
-
-type_synonym ('\<Sigma>\<^sub>t\<^sub>y, 'd) type_interp_fun = "'\<Sigma>\<^sub>t\<^sub>y \<Rightarrow> 'd set list \<Rightarrow> 'd set"
-type_synonym ('\<V>\<^sub>t\<^sub>y, 'd) type_valuation = "'\<V>\<^sub>t\<^sub>y \<Rightarrow> 'd set"
-
-type_synonym ('\<Sigma>, 'd) term_interp_fun = "'\<Sigma> \<Rightarrow> 'd set list \<Rightarrow> 'd list \<Rightarrow> 'd"
-type_synonym ('\<V>, 'd) term_valuation = "'\<V> \<Rightarrow> 'd"
-
-type_synonym ('\<V>\<^sub>t\<^sub>y, '\<Sigma>\<^sub>t\<^sub>y, '\<V>, '\<Sigma>, 'd) lambda_designation_fun =
-  "('\<V>\<^sub>t\<^sub>y, 'd) type_valuation \<Rightarrow> ('\<V>, 'd) term_valuation \<Rightarrow> (('\<V>\<^sub>t\<^sub>y, '\<Sigma>\<^sub>t\<^sub>y) ty, '\<Sigma>, '\<V>) preterm \<Rightarrow> 'd"
-
-type_synonym ('\<V>\<^sub>t\<^sub>y, '\<Sigma>\<^sub>t\<^sub>y, '\<V>, '\<Sigma>, 'd) interp =
-  "('\<Sigma>\<^sub>t\<^sub>y, 'd) type_interp_fun \<times>
-    ('\<Sigma>, 'd) term_interp_fun \<times>
-    ('\<V>\<^sub>t\<^sub>y, '\<Sigma>\<^sub>t\<^sub>y, '\<V>, '\<Sigma>, 'd) lambda_designation_fun"
-type_synonym ('\<V>\<^sub>t\<^sub>y, '\<V>, 'd) valuation =
-  "('\<V>\<^sub>t\<^sub>y, 'd) type_valuation \<times> ('\<V>, 'd) term_valuation"
-
-type_synonym ('\<V>\<^sub>t\<^sub>y, '\<Sigma>\<^sub>t\<^sub>y, '\<V>, '\<Sigma>, 'd) model =
-  "('\<V>\<^sub>t\<^sub>y, '\<Sigma>\<^sub>t\<^sub>y, '\<V>, '\<Sigma>, 'd) interp \<times> ('\<V>\<^sub>t\<^sub>y, '\<V>, 'd) valuation"
-
-locale type_interp =
-  fixes \<J>\<^sub>t\<^sub>y :: "('\<Sigma>\<^sub>t\<^sub>y :: arity, 'd :: domain_universe) type_interp_fun"
-  assumes \<J>\<^sub>t\<^sub>y_codom: "\<And>\<kappa> \<D>s.
-    arity \<kappa> = length \<D>s \<Longrightarrow> (\<And>\<D>. \<D> \<in> set \<D>s \<Longrightarrow> \<D> \<in> \<U>) \<Longrightarrow> \<J>\<^sub>t\<^sub>y \<kappa> \<D>s \<in> \<U>"
-
-primrec prety_denotation ::
-  "('\<V>\<^sub>t\<^sub>y, 'd) type_valuation \<Rightarrow> ('\<Sigma>\<^sub>t\<^sub>y, 'd) type_interp_fun \<Rightarrow> ('\<V>\<^sub>t\<^sub>y, '\<Sigma>\<^sub>t\<^sub>y) prety \<Rightarrow> 'd set" where
-  "prety_denotation \<xi>\<^sub>t\<^sub>y \<J>\<^sub>t\<^sub>y (PretyVar x) = \<xi>\<^sub>t\<^sub>y x" |
-  "prety_denotation \<xi>\<^sub>t\<^sub>y \<J>\<^sub>t\<^sub>y (PretyCtr \<kappa> \<tau>s) = \<J>\<^sub>t\<^sub>y \<kappa> (map (prety_denotation \<xi>\<^sub>t\<^sub>y \<J>\<^sub>t\<^sub>y) \<tau>s)"
-
-definition ty_denotation ::
-  "('\<V>\<^sub>t\<^sub>y, 'd) type_valuation \<Rightarrow> ('\<Sigma>\<^sub>t\<^sub>y, 'd) type_interp_fun \<Rightarrow> ('\<V>\<^sub>t\<^sub>y, '\<Sigma>\<^sub>t\<^sub>y :: arity) ty \<Rightarrow> 'd set" where
-  "ty_denotation \<xi>\<^sub>t\<^sub>y \<J>\<^sub>t\<^sub>y \<tau> = prety_denotation \<xi>\<^sub>t\<^sub>y \<J>\<^sub>t\<^sub>y (Rep_ty \<tau>)"
-
-locale type_valuation =
-  fixes \<xi>\<^sub>t\<^sub>y :: "('\<V>\<^sub>t\<^sub>y, 'd :: domain_universe) type_valuation"
-  assumes \<xi>\<^sub>t\<^sub>y_codom[intro]: "\<And>x. \<xi>\<^sub>t\<^sub>y x \<in> \<U>"
-
-lemma ty_denotation_codom:
-  assumes "type_interp \<J>\<^sub>t\<^sub>y" and "type_valuation \<xi>\<^sub>t\<^sub>y"
-  shows "ty_denotation \<xi>\<^sub>t\<^sub>y \<J>\<^sub>t\<^sub>y \<tau> \<in> \<U>"
-proof (cases \<tau>)
-  case (Abs_ty \<tau>')
-
-  then have "wf_prety \<tau>'"
-    by simp
-
-  then have "prety_denotation \<xi>\<^sub>t\<^sub>y \<J>\<^sub>t\<^sub>y \<tau>' \<in> \<U>"
-  proof (induction \<tau>')
-    case (PretyVar \<alpha>)
-    then show ?case
-      by (metis assms(2) prety_denotation.simps(1) type_valuation.\<xi>\<^sub>t\<^sub>y_codom)
-  next
-    case (PretyCtr \<kappa> \<tau>s)
-    show ?case
-      unfolding prety_denotation.simps
-    proof (rule type_interp.\<J>\<^sub>t\<^sub>y_codom[OF assms(1)])
-      show "arity \<kappa> = length (map (prety_denotation \<xi>\<^sub>t\<^sub>y \<J>\<^sub>t\<^sub>y) \<tau>s)"
-        using PretyCtr.hyps by simp
-    next
-      show "\<And>\<D>. \<D> \<in> set (map (prety_denotation \<xi>\<^sub>t\<^sub>y \<J>\<^sub>t\<^sub>y) \<tau>s) \<Longrightarrow> \<D> \<in> \<U>"
-        using PretyCtr.IH by auto
-    qed
-  qed
-
-  then show ?thesis
-    using Abs_ty
-    by (metis Abs_ty_inverse[of \<tau>'] ty_denotation_def)
-qed
-
-locale interp_fun = type_interp \<J>\<^sub>t\<^sub>y
-  for \<J>\<^sub>t\<^sub>y :: "('\<Sigma>\<^sub>t\<^sub>y :: arity, 'd :: domain_universe) type_interp_fun" +
-  fixes typeof :: "'\<Sigma> \<Rightarrow> ('\<V>\<^sub>t\<^sub>y, '\<Sigma>\<^sub>t\<^sub>y) const_ty"
-  fixes \<J> :: "('\<Sigma>, 'd) term_interp_fun"
-  assumes
-    \<J>_codom[intro]: "\<And>(\<xi>\<^sub>t\<^sub>y :: ('\<V>\<^sub>t\<^sub>y, 'd) type_valuation) \<kappa> \<D>s \<alpha>s \<tau>s \<pi> as.
-      type_valuation \<xi>\<^sub>t\<^sub>y \<Longrightarrow>
-      typeof \<kappa> = (\<alpha>s, \<tau>s, \<pi>) \<Longrightarrow> Dlist.length \<alpha>s = length \<D>s \<Longrightarrow>
-      list_all2 (\<lambda>a \<tau>. a \<in> ty_denotation \<xi>\<^sub>t\<^sub>y \<J>\<^sub>t\<^sub>y \<tau>) as \<tau>s \<Longrightarrow> \<J> \<kappa> \<D>s as \<in> ty_denotation \<xi>\<^sub>t\<^sub>y \<J>\<^sub>t\<^sub>y \<pi>"
-
-locale valuation =
-  fixes typeof_var :: "'\<V> \<Rightarrow> ('\<V>\<^sub>t\<^sub>y, '\<Sigma>\<^sub>t\<^sub>y :: arity) ty"
-  fixes \<xi> :: "('\<V>, 'd :: domain_universe) term_valuation"
-  assumes \<xi>_codom[intro]: "\<And>(\<xi>\<^sub>t\<^sub>y :: ('\<V>\<^sub>t\<^sub>y, 'd) type_valuation) x.
-    type_valuation \<xi>\<^sub>t\<^sub>y \<Longrightarrow> \<xi> x \<in> ty_denotation \<xi>\<^sub>t\<^sub>y \<J>\<^sub>t\<^sub>y (typeof_var x)"
-
-locale lambda_designation = type_interp \<J>\<^sub>t\<^sub>y
-  for \<J>\<^sub>t\<^sub>y :: "('\<Sigma>\<^sub>t\<^sub>y :: type_signature, 'd :: domain_universe) type_interp_fun" +
-  fixes typeof :: "'\<Sigma> \<Rightarrow> ('\<V>\<^sub>t\<^sub>y, '\<Sigma>\<^sub>t\<^sub>y) const_ty"
-  fixes \<L> :: "('\<V>\<^sub>t\<^sub>y, '\<Sigma>\<^sub>t\<^sub>y, '\<V>, '\<Sigma>, 'd) lambda_designation_fun"
-  assumes "\<And>(\<xi>\<^sub>t\<^sub>y :: ('\<V>\<^sub>t\<^sub>y, 'd) type_valuation) (\<xi> :: ('\<V>, 'd) term_valuation) (typeof_var :: '\<V> \<Rightarrow> ('\<V>\<^sub>t\<^sub>y, '\<Sigma>\<^sub>t\<^sub>y) ty) t \<tau>.
-    type_valuation \<xi>\<^sub>t\<^sub>y \<Longrightarrow>
-    has_type typeof typeof_var t \<tau> \<Longrightarrow> is_Abs t \<Longrightarrow> \<L> \<xi>\<^sub>t\<^sub>y \<xi> t \<in> ty_denotation \<xi>\<^sub>t\<^sub>y \<J>\<^sub>t\<^sub>y \<tau>"
-  assumes \<L>_depends_only_on_\<xi>_on_vars:
-    "\<And>(\<xi>\<^sub>t\<^sub>y :: ('\<V>\<^sub>t\<^sub>y, 'd) type_valuation) (\<xi>\<^sub>t\<^sub>y' :: ('\<V>\<^sub>t\<^sub>y, 'd) type_valuation)
-      (\<xi> :: ('\<V>, 'd) term_valuation) (\<xi>' :: ('\<V>, 'd) term_valuation) t.
-    (\<And>\<tau> x. \<tau> \<in> type_symbols t \<Longrightarrow> x \<in> type_vars \<tau> \<Longrightarrow> \<xi>\<^sub>t\<^sub>y x = \<xi>\<^sub>t\<^sub>y' x) \<Longrightarrow>
-    (\<And>x. x \<in> free_vars t \<Longrightarrow> \<xi> x = \<xi>' x) \<Longrightarrow> \<L> \<xi>\<^sub>t\<^sub>y \<xi> t = \<L> \<xi>\<^sub>t\<^sub>y' \<xi>' t"
-
-locale interp =
-  type_interp \<J>\<^sub>t\<^sub>y +
-  interp_fun \<J>\<^sub>t\<^sub>y typeof \<J> +
-  lambda_designation \<J>\<^sub>t\<^sub>y typeof \<L>
-  for
-    \<J>\<^sub>t\<^sub>y :: "('\<Sigma>\<^sub>t\<^sub>y :: type_signature, 'd :: domain_universe) type_interp_fun" and
-    typeof :: "'\<Sigma> \<Rightarrow> ('\<V>\<^sub>t\<^sub>y, '\<Sigma>\<^sub>t\<^sub>y) const_ty" and
-    \<J> :: "('\<Sigma>, 'd) term_interp_fun" and
-    \<L> :: "('\<V>\<^sub>t\<^sub>y, '\<Sigma>\<^sub>t\<^sub>y, '\<V>, '\<Sigma>, 'd) lambda_designation_fun"
-
-primrec preterm_denotation ::
-  "('\<V>\<^sub>t\<^sub>y, 'd :: domain_universe) type_valuation \<Rightarrow> ('\<V>, 'd) term_valuation \<Rightarrow>
-    ('\<Sigma>\<^sub>t\<^sub>y :: arity, 'd) type_interp_fun \<Rightarrow> ('\<Sigma>, 'd) term_interp_fun \<Rightarrow>
-    ('\<V>\<^sub>t\<^sub>y, '\<Sigma>\<^sub>t\<^sub>y, '\<V>, '\<Sigma>, 'd) lambda_designation_fun \<Rightarrow>
-    (('\<V>\<^sub>t\<^sub>y, '\<Sigma>\<^sub>t\<^sub>y) ty, '\<Sigma>, '\<V>) preterm \<Rightarrow> 'd" where
-  "preterm_denotation \<xi>\<^sub>t\<^sub>y \<xi> \<J>\<^sub>t\<^sub>y \<J> \<L> (Free x) = \<xi> x" |
-  "preterm_denotation \<xi>\<^sub>t\<^sub>y \<xi> \<J>\<^sub>t\<^sub>y \<J> \<L> (Const f \<tau>s ts) =
-    \<J> f (map (ty_denotation \<xi>\<^sub>t\<^sub>y \<J>\<^sub>t\<^sub>y) \<tau>s) (map (preterm_denotation \<xi>\<^sub>t\<^sub>y \<xi> \<J>\<^sub>t\<^sub>y \<J> \<L>) ts)" |
-  "preterm_denotation \<xi>\<^sub>t\<^sub>y \<xi> \<J>\<^sub>t\<^sub>y \<J> \<L> (App t\<^sub>1 t\<^sub>2) = ap_domain (preterm_denotation \<xi>\<^sub>t\<^sub>y \<xi> \<J>\<^sub>t\<^sub>y \<J> \<L> t\<^sub>1) (preterm_denotation \<xi>\<^sub>t\<^sub>y \<xi> \<J>\<^sub>t\<^sub>y \<J> \<L> t\<^sub>1)" |
-  "preterm_denotation \<xi>\<^sub>t\<^sub>y \<xi> \<J>\<^sub>t\<^sub>y \<J> \<L> (Abs \<tau> t) = \<L> \<xi>\<^sub>t\<^sub>y \<xi> (Abs \<tau> t)" |
-  "preterm_denotation \<xi>\<^sub>t\<^sub>y \<xi> \<J>\<^sub>t\<^sub>y \<J> \<L> (Bound _) = undefined"
-
-lemma (in type_interp) ty_denotation_of_ground:
-  assumes "type_vars \<tau> = {}"
-  shows "ty_denotation \<xi>\<^sub>t\<^sub>y \<J>\<^sub>t\<^sub>y \<tau> = ty_denotation \<xi>\<^sub>t\<^sub>y' \<J>\<^sub>t\<^sub>y \<tau>"
-proof (cases \<tau>)
-  case (Abs_ty \<tau>')
-
-  then have "type_vars_prety \<tau>' = {}"
-    using assms
-    by (metis Abs_ty_inverse type_vars.rep_eq)
-
-  then have "prety_denotation \<xi>\<^sub>t\<^sub>y \<J>\<^sub>t\<^sub>y \<tau>' = prety_denotation \<xi>\<^sub>t\<^sub>y' \<J>\<^sub>t\<^sub>y \<tau>'"
-  proof (induction \<tau>')
-    case (PretyVar x)
-    then have False
-      by simp
-
-    then show ?case ..
-  next
-    case (PretyCtr \<kappa> \<pi>s)
-
-    then have "\<pi> \<in> set \<pi>s \<Longrightarrow> prety_denotation \<xi>\<^sub>t\<^sub>y \<J>\<^sub>t\<^sub>y \<pi> = prety_denotation \<xi>\<^sub>t\<^sub>y' \<J>\<^sub>t\<^sub>y \<pi>"
-      for \<pi>
-      by simp
-
-    then show ?case
-      by (metis (no_types, lifting) map_eq_conv prety_denotation.simps(2))
-  qed
-
-  then show ?thesis
-    using Abs_ty
-    by (metis Abs_ty_inverse ty_denotation_def)
-qed
-
-lemma (in interp)
-  assumes "free_vars t = {}" and "(\<Union>\<tau> \<in> type_symbols t. type_vars \<tau>) = {}"
-  shows "preterm_denotation \<xi>\<^sub>t\<^sub>y \<xi> \<J>\<^sub>t\<^sub>y \<J> \<L> t = preterm_denotation \<xi>\<^sub>t\<^sub>y' \<xi>' \<J>\<^sub>t\<^sub>y \<J> \<L> t"
-  using assms
-proof (induction t)
-  case (Const f \<tau>s ts)
-
-  then have IH': "preterm_denotation \<xi>\<^sub>t\<^sub>y \<xi> \<J>\<^sub>t\<^sub>y \<J> \<L> t = preterm_denotation \<xi>\<^sub>t\<^sub>y' \<xi>' \<J>\<^sub>t\<^sub>y \<J> \<L> t"
-    if "t \<in> set ts" for t
-    by (simp add: that)
-
-  then have "\<J> f (map (ty_denotation \<xi>\<^sub>t\<^sub>y \<J>\<^sub>t\<^sub>y) \<tau>s) (map (preterm_denotation \<xi>\<^sub>t\<^sub>y \<xi> \<J>\<^sub>t\<^sub>y \<J> \<L>) ts) =
-    \<J> f (map (ty_denotation \<xi>\<^sub>t\<^sub>y' \<J>\<^sub>t\<^sub>y) \<tau>s) (map (preterm_denotation \<xi>\<^sub>t\<^sub>y' \<xi>' \<J>\<^sub>t\<^sub>y \<J> \<L>) ts)"
-    using ty_denotation_of_ground
-    by (metis (mono_tags, lifting) Const.prems(2)
-        UNION_empty_conv(1) list.map_cong0[of \<tau>s] list.map_cong0[of ts]
-        preterm.set_intros(1))
-
-  then show ?case
-    by simp
-next
-  case (Abs \<tau> t)
-  have "\<L> \<xi>\<^sub>t\<^sub>y \<xi> (Abs \<tau> t) = \<L> \<xi>\<^sub>t\<^sub>y' \<xi>' (Abs \<tau> t)"
-  proof (rule \<L>_depends_only_on_\<xi>_on_vars)
-    show "\<And>\<tau>' x. \<tau>' \<in> type_symbols (Abs \<tau> t) \<Longrightarrow> x \<in> type_vars \<tau>' \<Longrightarrow> \<xi>\<^sub>t\<^sub>y x = \<xi>\<^sub>t\<^sub>y' x"
-      using Abs.prems(2) by blast
-  next
-    show "\<And>x. x \<in> free_vars (Abs \<tau> t) \<Longrightarrow> \<xi> x = \<xi>' x"
-      by (metis Abs.prems(1) emptyE)
-  qed
-
-  then show ?case
-    by simp
-qed simp_all
-
-locale proper_interp = interp +
-  assumes "ap_domain (\<L> \<xi>\<^sub>t\<^sub>y \<xi> (Abs \<tau> t)) a = \<L> \<xi>\<^sub>t\<^sub>y (\<xi>(x := a)) (subst_bound 0 (Free x) t)"
-
-type_synonym ('\<V>\<^sub>t\<^sub>y, '\<Sigma>\<^sub>t\<^sub>y, '\<V>, '\<Sigma>) atom = "(('\<V>\<^sub>t\<^sub>y, '\<Sigma>\<^sub>t\<^sub>y) ty, '\<Sigma>, '\<V>) preterm uprod"
-datatype 'a literal =
-  is_pos: Pos (atm: 'a) |
-  is_neg: Neg (atm: 'a)
-
-instantiation literal :: (type) uminus
-begin
-
-primrec uminus_literal :: "'a literal \<Rightarrow> 'a literal" where
-  "uminus (Pos A) = Neg A" |
-  "uminus (Neg A) = Pos A"
-
-instance ..
-
-end
-
-fun true_lit ::
-  "('\<V>\<^sub>t\<^sub>y, '\<Sigma>\<^sub>t\<^sub>y :: arity, '\<V>, '\<Sigma>, 'd :: domain_universe) model \<Rightarrow> ('\<V>\<^sub>t\<^sub>y, '\<Sigma>\<^sub>t\<^sub>y, '\<V>, '\<Sigma>) atom literal \<Rightarrow> bool"
-  (infix \<open>\<Turnstile>\<^sub>l\<close> 50) where
-  "((\<J>\<^sub>t\<^sub>y, \<J>, \<L>), (\<xi>\<^sub>t\<^sub>y, \<xi>)) \<Turnstile>\<^sub>l (Pos A) \<longleftrightarrow>
-    case_uprod (Abs_commute (=)) (map_uprod (preterm_denotation \<xi>\<^sub>t\<^sub>y \<xi> \<J>\<^sub>t\<^sub>y \<J> \<L>) A)" |
-  "((\<J>\<^sub>t\<^sub>y, \<J>, \<L>), (\<xi>\<^sub>t\<^sub>y, \<xi>)) \<Turnstile>\<^sub>l (Neg A) \<longleftrightarrow>
-    case_uprod (Abs_commute (\<noteq>)) (map_uprod (preterm_denotation \<xi>\<^sub>t\<^sub>y \<xi> \<J>\<^sub>t\<^sub>y \<J> \<L>) A)"
-
-lemma model_exhaust[case_names Model]:
-  fixes \<M> :: "('\<V>\<^sub>t\<^sub>y, '\<Sigma>\<^sub>t\<^sub>y, '\<V>, '\<Sigma>, 'd) model" and P :: bool
-  assumes "\<And>\<J>\<^sub>t\<^sub>y \<J> \<L> \<xi>\<^sub>t\<^sub>y \<xi>. \<M> = ((\<J>\<^sub>t\<^sub>y, \<J>, \<L>), (\<xi>\<^sub>t\<^sub>y, \<xi>)) \<Longrightarrow> P"
-  shows P
-  using assms
-  by (metis prod.exhaust)
 
 lemma apply_commute_Abs_commute_ident_if_commutative[simp]:
   assumes commutative: "\<And>x y. R x y = R y x"
@@ -242,155 +17,295 @@ lemma apply_commute_Abs_commute_ident_if_eq[simp]:
   shows "apply_commute (Abs_commute (\<lambda>x y. (f x) = (f y))) = (\<lambda>x y. (f x) = (f y))"
   using apply_commute_Abs_commute_ident_if_commutative[of "(=)" f] by metis
 
+lemma apply_commute_Abs_commute_eq[simp]: "apply_commute (Abs_commute (=)) = (=)"
+proof (rule apply_commute_Abs_commute_ident_if_commutative)
+  show "\<And>x y. (x = y) = (y = x)"
+    by metis
+qed
+
+lemma apply_commute_Abs_commute_neq[simp]: "apply_commute (Abs_commute (\<noteq>)) = (\<noteq>)"
+proof (rule apply_commute_Abs_commute_ident_if_commutative)
+  show "\<And>x y. (x \<noteq> y) = (y \<noteq> x)"
+    by metis
+qed
+
 lemma case_uprod_Abs_commute_neq[simp]:
   "case_uprod (Abs_commute (\<noteq>)) p \<longleftrightarrow> \<not> case_uprod (Abs_commute (=)) p"
-  by (smt (verit) Abs_commute_inverse CollectI
-      case_uprod_simps uprod_exhaust)
+  by (smt (verit) Abs_commute_inverse CollectI case_uprod_simps uprod_exhaust)
 
-lemma true_lit_iff_not_true_uminus_lit[simp]: "\<not> (\<M> \<Turnstile>\<^sub>l L) \<longleftrightarrow> \<M> \<Turnstile>\<^sub>l -L"
-proof (cases \<M> rule: model_exhaust)
-  case (Model \<J>\<^sub>t\<^sub>y \<J> \<L> \<xi>\<^sub>t\<^sub>y \<xi>)
-  then show ?thesis
-    by (cases L) simp_all
+term funcset
+
+typ V
+
+find_consts "_ \<Rightarrow> V"
+
+term V_of
+term elts
+
+
+definition V_of :: "'a::embeddable \<Rightarrow> V"
+  where "V_of \<equiv> SOME f. inj f"
+
+abbreviation vfunspace :: "V \<Rightarrow> V \<Rightarrow> V"
+  where "vfunspace A B \<equiv> VPi A (\<lambda>_. B)"
+
+locale universe =
+  fixes \<U> :: "V set"
+  assumes nonempty_\<U>: "0 \<notin> \<U>"
+  assumes boolset_in_\<U>: "set {0,1} \<in> \<U>"
+
+type_synonym '\<Sigma>\<^sub>t\<^sub>y type_interp_fun = "'\<Sigma>\<^sub>t\<^sub>y \<Rightarrow> V list \<Rightarrow> V"
+
+locale type_interp = universe +
+  fixes \<J>\<^sub>t\<^sub>y :: "('\<Sigma>\<^sub>t\<^sub>y :: type_signature) type_interp_fun"
+  assumes
+    \<J>\<^sub>t\<^sub>y_codom[intro]: "\<And>\<D>s \<kappa>.
+      length \<D>s = arity \<kappa> \<Longrightarrow> (\<And>\<D>. \<D> \<in> list.set \<D>s \<Longrightarrow> \<D> \<in> \<U>) \<Longrightarrow> \<J>\<^sub>t\<^sub>y \<kappa> \<D>s \<in> \<U>" and
+    \<J>\<^sub>t\<^sub>y_bool[simp]: "\<J>\<^sub>t\<^sub>y bool_tyctr [] = set {0,1}" and
+    \<J>\<^sub>t\<^sub>y_fun[intro]: "\<And>\<D>\<^sub>1 \<D>\<^sub>2. \<D>\<^sub>1 \<in> \<U> \<Longrightarrow> \<D>\<^sub>2 \<in> \<U> \<Longrightarrow> \<J>\<^sub>t\<^sub>y fun_tyctr [\<D>\<^sub>1, \<D>\<^sub>2] \<le> vfunspace \<D>\<^sub>1 \<D>\<^sub>2"
+
+locale type_valuation = universe +
+  fixes \<xi>\<^sub>t\<^sub>y :: "'\<V>\<^sub>t\<^sub>y \<Rightarrow> V"
+  assumes \<xi>\<^sub>t\<^sub>y_codom[intro]: "\<And>x. \<xi>\<^sub>t\<^sub>y x \<in> \<U>"
+
+primrec denotation_prety ::
+  "('\<V>\<^sub>t\<^sub>y \<Rightarrow> V) \<Rightarrow> '\<Sigma>\<^sub>t\<^sub>y type_interp_fun \<Rightarrow> ('\<V>\<^sub>t\<^sub>y, '\<Sigma>\<^sub>t\<^sub>y) prety \<Rightarrow> V" where
+  "denotation_prety \<xi>\<^sub>t\<^sub>y \<J>\<^sub>t\<^sub>y (PretyVar \<alpha>) = \<xi>\<^sub>t\<^sub>y \<alpha>" |
+  "denotation_prety \<xi>\<^sub>t\<^sub>y \<J>\<^sub>t\<^sub>y (PretyCtr \<kappa> \<tau>s) = \<J>\<^sub>t\<^sub>y \<kappa> (map (denotation_prety \<xi>\<^sub>t\<^sub>y \<J>\<^sub>t\<^sub>y) \<tau>s)"
+
+definition denotation_ty ::
+  "('\<V>\<^sub>t\<^sub>y \<Rightarrow> V) \<Rightarrow> '\<Sigma>\<^sub>t\<^sub>y type_interp_fun \<Rightarrow> ('\<V>\<^sub>t\<^sub>y, '\<Sigma>\<^sub>t\<^sub>y :: arity) ty \<Rightarrow> V" where
+  "denotation_ty \<xi>\<^sub>t\<^sub>y \<J>\<^sub>t\<^sub>y \<tau> = denotation_prety \<xi>\<^sub>t\<^sub>y \<J>\<^sub>t\<^sub>y (Rep_ty \<tau>)"
+
+lemma
+  assumes "type_interp \<U> \<J>\<^sub>t\<^sub>y" and "type_valuation \<U> \<xi>\<^sub>t\<^sub>y"
+  shows
+    denotation_prety_in_universe: "\<And>\<tau>. wf_prety \<tau> \<Longrightarrow> denotation_prety \<xi>\<^sub>t\<^sub>y \<J>\<^sub>t\<^sub>y \<tau> \<in> \<U>" and
+    denotation_ty_in_universe: "\<And>\<tau>. denotation_ty \<xi>\<^sub>t\<^sub>y \<J>\<^sub>t\<^sub>y \<tau> \<in> \<U>"
+proof -
+  show 1: "denotation_prety \<xi>\<^sub>t\<^sub>y \<J>\<^sub>t\<^sub>y \<tau> \<in> \<U>" if "wf_prety \<tau>" for \<tau>
+    using that
+  proof (induction \<tau>)
+    case (PretyVar \<alpha>)
+    then show ?case
+      by (metis assms(2) denotation_prety.simps(1) type_valuation.\<xi>\<^sub>t\<^sub>y_codom)
+  next
+    case (PretyCtr \<kappa> \<tau>s)
+    show ?case
+      unfolding denotation_prety.simps
+    proof (rule type_interp.\<J>\<^sub>t\<^sub>y_codom[OF assms(1)])
+      show "length (map (denotation_prety \<xi>\<^sub>t\<^sub>y \<J>\<^sub>t\<^sub>y) \<tau>s) = arity \<kappa>"
+        using PretyCtr.hyps by simp
+    next
+      show "\<And>\<D>. \<D> \<in> list.set (map (denotation_prety \<xi>\<^sub>t\<^sub>y \<J>\<^sub>t\<^sub>y) \<tau>s) \<Longrightarrow> \<D> \<in> \<U>"
+        using PretyCtr.IH by auto
+    qed
+  qed
+
+  show "denotation_ty \<xi>\<^sub>t\<^sub>y \<J>\<^sub>t\<^sub>y \<tau> \<in> \<U>" for \<tau>
+  proof (cases \<tau>)
+    case (Abs_ty \<tau>')
+    then have "wf_prety \<tau>'"
+      by simp
+    then have "denotation_prety \<xi>\<^sub>t\<^sub>y \<J>\<^sub>t\<^sub>y \<tau>' \<in> \<U>"
+      using 1 by iprover
+    then show ?thesis
+      using Abs_ty
+      by (metis Abs_ty_inverse[of \<tau>'] denotation_ty_def)
+  qed
 qed
 
-lemma true_lit_Pos_ident: "\<M> \<Turnstile>\<^sub>l (Pos (Upair t t))"
-proof (cases \<M> rule: model_exhaust)
-  case (Model \<J>\<^sub>t\<^sub>y \<J> \<L> \<xi>\<^sub>t\<^sub>y \<xi>)
+locale term_valuation = type_interp \<U> \<J>\<^sub>t\<^sub>y + type_valuation \<U> \<xi>\<^sub>t\<^sub>y for  \<U> \<J>\<^sub>t\<^sub>y \<xi>\<^sub>t\<^sub>y +
+  fixes \<xi>\<^sub>t\<^sub>e :: "'\<V>\<^sub>t\<^sub>e \<Rightarrow> V"
+  assumes \<xi>\<^sub>t\<^sub>e_codom[intro]: "\<And>x \<tau>. \<xi>\<^sub>t\<^sub>e x \<in> elts (denotation_ty \<xi>\<^sub>t\<^sub>y \<J>\<^sub>t\<^sub>y \<tau>)"
+
+locale valuation = type_valuation \<U> \<xi>\<^sub>t\<^sub>y + term_valuation \<U> \<J>\<^sub>t\<^sub>y \<xi>\<^sub>t\<^sub>y \<xi>\<^sub>t\<^sub>e
+  for \<U> \<J>\<^sub>t\<^sub>y \<xi>\<^sub>t\<^sub>y \<xi>\<^sub>t\<^sub>e
+
+type_synonym '\<Sigma> term_interp_fun = "'\<Sigma> \<Rightarrow> V list \<Rightarrow> V list \<Rightarrow> V"
+
+locale interp_fun = type_interp \<U> \<J>\<^sub>t\<^sub>y
+  for \<U> and \<J>\<^sub>t\<^sub>y :: "('\<Sigma>\<^sub>t\<^sub>y :: type_signature) type_interp_fun" +
+  fixes \<C> :: "'\<Sigma> \<Rightarrow> ('\<V>\<^sub>t\<^sub>y, '\<Sigma>\<^sub>t\<^sub>y) const_ty"
+  fixes \<J> :: "'\<Sigma> term_interp_fun"
+  assumes "\<And>(\<xi>\<^sub>t\<^sub>y :: '\<V>\<^sub>t\<^sub>y \<Rightarrow> V) f \<alpha>s \<tau>s v \<D>s as.
+    type_valuation \<U> \<xi>\<^sub>t\<^sub>y \<Longrightarrow>
+    \<C> f = (\<alpha>s, \<tau>s, v) \<Longrightarrow> length \<D>s = Dlist.length \<alpha>s \<Longrightarrow>
+    (\<And>\<D>. \<D> \<in> list.set \<D>s \<Longrightarrow> \<D> \<in> \<U>) \<Longrightarrow>
+    list_all2 (\<lambda>a \<tau>. a \<in> elts (denotation_ty \<xi>\<^sub>t\<^sub>y \<J>\<^sub>t\<^sub>y \<tau>)) as \<tau>s \<Longrightarrow>
+    \<J> f \<D>s as \<in> elts (denotation_ty \<xi>\<^sub>t\<^sub>y \<J>\<^sub>t\<^sub>y v)"
+
+type_synonym ('\<V>\<^sub>t\<^sub>y, '\<Sigma>\<^sub>t\<^sub>y, '\<V>, '\<Sigma>) lambda_designation_fun =
+  "('\<V>\<^sub>t\<^sub>y \<Rightarrow> V) \<Rightarrow> ('\<V> \<Rightarrow> V) \<Rightarrow> (('\<V>\<^sub>t\<^sub>y, '\<Sigma>\<^sub>t\<^sub>y) ty, '\<Sigma>, '\<V>) preterm \<Rightarrow> V"
+
+locale lambda_designation = type_interp \<U> \<J>\<^sub>t\<^sub>y
+  for \<U> and \<J>\<^sub>t\<^sub>y :: "('\<Sigma>\<^sub>t\<^sub>y :: type_signature) type_interp_fun" +
+  fixes \<C> :: "'\<Sigma> \<Rightarrow> ('\<V>\<^sub>t\<^sub>y, '\<Sigma>\<^sub>t\<^sub>y) const_ty"
+  fixes \<L> :: "('\<V>\<^sub>t\<^sub>y, '\<Sigma>\<^sub>t\<^sub>y, '\<V>, '\<Sigma>) lambda_designation_fun"
+  assumes "\<And>(\<xi>\<^sub>t\<^sub>y :: '\<V>\<^sub>t\<^sub>y \<Rightarrow> V) (\<xi>\<^sub>t\<^sub>e :: '\<V> \<Rightarrow> V) (\<F> :: '\<V> \<Rightarrow> ('\<V>\<^sub>t\<^sub>y, '\<Sigma>\<^sub>t\<^sub>y) ty) t \<tau>.
+    type_valuation \<U> \<xi>\<^sub>t\<^sub>y \<Longrightarrow> term_valuation \<U> \<J>\<^sub>t\<^sub>y \<xi>\<^sub>t\<^sub>y \<xi>\<^sub>t\<^sub>e \<Longrightarrow>
+    has_type \<C> \<F> t \<tau> \<Longrightarrow> is_Abs t \<Longrightarrow>
+    \<L> \<xi>\<^sub>t\<^sub>y \<xi>\<^sub>t\<^sub>e t \<in> elts (denotation_ty \<xi>\<^sub>t\<^sub>y \<J>\<^sub>t\<^sub>y \<tau>)"
+  assumes \<L>_depends_only_on_\<xi>_on_vars:
+    "\<And>(\<xi>\<^sub>t\<^sub>y :: '\<V>\<^sub>t\<^sub>y \<Rightarrow> V) (\<xi>\<^sub>t\<^sub>y' :: '\<V>\<^sub>t\<^sub>y \<Rightarrow> V) (\<xi>\<^sub>t\<^sub>e :: '\<V> \<Rightarrow> V) (\<xi>\<^sub>t\<^sub>e' :: '\<V> \<Rightarrow> V) t.
+    (\<And>\<tau> x. \<tau> \<in> type_symbols t \<Longrightarrow> x \<in> type_vars \<tau> \<Longrightarrow> \<xi>\<^sub>t\<^sub>y x = \<xi>\<^sub>t\<^sub>y' x) \<Longrightarrow>
+    (\<And>x. x \<in> free_vars t \<Longrightarrow> \<xi>\<^sub>t\<^sub>e x = \<xi>\<^sub>t\<^sub>e' x) \<Longrightarrow> \<L> \<xi>\<^sub>t\<^sub>y \<xi>\<^sub>t\<^sub>e t = \<L> \<xi>\<^sub>t\<^sub>y' \<xi>\<^sub>t\<^sub>e' t"
+
+locale interp =
+  type_interp \<U> \<J>\<^sub>t\<^sub>y +
+  interp_fun \<U> \<J>\<^sub>t\<^sub>y \<C> \<J> +
+  lambda_designation \<U> \<J>\<^sub>t\<^sub>y \<C> \<L>
+  for \<U> and
+    \<J>\<^sub>t\<^sub>y :: "('\<Sigma>\<^sub>t\<^sub>y :: type_signature) type_interp_fun" and
+    \<C> :: "'\<Sigma> \<Rightarrow> ('\<V>\<^sub>t\<^sub>y, '\<Sigma>\<^sub>t\<^sub>y) const_ty" and
+    \<J> :: "'\<Sigma> term_interp_fun" and
+    \<L> :: "('\<V>\<^sub>t\<^sub>y, '\<Sigma>\<^sub>t\<^sub>y, '\<V>, '\<Sigma>) lambda_designation_fun"
+
+primrec denotation_preterm ::
+  "('\<V>\<^sub>t\<^sub>y \<Rightarrow> V) \<Rightarrow> ('\<V> \<Rightarrow> V) \<Rightarrow>
+    ('\<Sigma>\<^sub>t\<^sub>y :: arity) type_interp_fun \<Rightarrow> '\<Sigma> term_interp_fun \<Rightarrow>
+    ('\<V>\<^sub>t\<^sub>y, '\<Sigma>\<^sub>t\<^sub>y, '\<V>, '\<Sigma>) lambda_designation_fun \<Rightarrow>
+    (('\<V>\<^sub>t\<^sub>y, '\<Sigma>\<^sub>t\<^sub>y) ty, '\<Sigma>, '\<V>) preterm \<Rightarrow> V" where
+  "denotation_preterm \<xi>\<^sub>t\<^sub>y \<xi>\<^sub>t\<^sub>e \<J>\<^sub>t\<^sub>y \<J> \<L> (Free x) = \<xi>\<^sub>t\<^sub>e x" |
+  "denotation_preterm \<xi>\<^sub>t\<^sub>y \<xi>\<^sub>t\<^sub>e \<J>\<^sub>t\<^sub>y \<J> \<L> (Const f \<tau>s ts) =
+    \<J> f (map (denotation_ty \<xi>\<^sub>t\<^sub>y \<J>\<^sub>t\<^sub>y) \<tau>s) (map (denotation_preterm \<xi>\<^sub>t\<^sub>y \<xi>\<^sub>t\<^sub>e \<J>\<^sub>t\<^sub>y \<J> \<L>) ts)" |
+  "denotation_preterm \<xi>\<^sub>t\<^sub>y \<xi>\<^sub>t\<^sub>e \<J>\<^sub>t\<^sub>y \<J> \<L> (App t\<^sub>1 t\<^sub>2) =
+    app (denotation_preterm \<xi>\<^sub>t\<^sub>y \<xi>\<^sub>t\<^sub>e \<J>\<^sub>t\<^sub>y \<J> \<L> t\<^sub>1) (denotation_preterm \<xi>\<^sub>t\<^sub>y \<xi>\<^sub>t\<^sub>e \<J>\<^sub>t\<^sub>y \<J> \<L> t\<^sub>1)" |
+  "denotation_preterm \<xi>\<^sub>t\<^sub>y \<xi>\<^sub>t\<^sub>e \<J>\<^sub>t\<^sub>y \<J> \<L> (Abs \<tau> t) = \<L> \<xi>\<^sub>t\<^sub>y \<xi>\<^sub>t\<^sub>e (Abs \<tau> t)" |
+  "denotation_preterm \<xi>\<^sub>t\<^sub>y \<xi>\<^sub>t\<^sub>e \<J>\<^sub>t\<^sub>y \<J> \<L> (Bound x) = undefined"
+
+
+subsection \<open>Denotation of ground terms\<close>
+
+lemma (in type_interp) denotation_ty_of_ground:
+  assumes "type_vars \<tau> = {}"
+  shows "denotation_ty \<xi>\<^sub>t\<^sub>y \<J>\<^sub>t\<^sub>y \<tau> = denotation_ty \<xi>\<^sub>t\<^sub>y' \<J>\<^sub>t\<^sub>y \<tau>"
+proof (cases \<tau>)
+  case (Abs_ty \<tau>')
+
+  then have "type_vars_prety \<tau>' = {}"
+    using assms
+    by (metis Abs_ty_inverse type_vars.rep_eq)
+
+  then have "denotation_prety \<xi>\<^sub>t\<^sub>y \<J>\<^sub>t\<^sub>y \<tau>' = denotation_prety \<xi>\<^sub>t\<^sub>y' \<J>\<^sub>t\<^sub>y \<tau>'"
+  proof (induction \<tau>')
+    case (PretyVar x)
+    then have False
+      by simp
+    then show ?case ..
+  next
+    case (PretyCtr \<kappa> \<pi>s)
+    then have "denotation_prety \<xi>\<^sub>t\<^sub>y \<J>\<^sub>t\<^sub>y \<pi> = denotation_prety \<xi>\<^sub>t\<^sub>y' \<J>\<^sub>t\<^sub>y \<pi>"
+      if "\<pi> \<in> list.set \<pi>s" for \<pi>
+      using that by simp
+    then show ?case
+      by (metis (no_types, lifting) map_eq_conv denotation_prety.simps(2))
+  qed
+
   then show ?thesis
+    using Abs_ty
+    by (simp add: Abs_ty_inverse denotation_ty_def)
+qed
+
+lemma (in interp) denotation_preterm_of_ground:
+  assumes "free_vars t = {}" and "(\<Union>\<tau> \<in> type_symbols t. type_vars \<tau>) = {}"
+  shows "denotation_preterm \<xi>\<^sub>t\<^sub>y \<xi>\<^sub>t\<^sub>e \<J>\<^sub>t\<^sub>y \<J> \<L> t = denotation_preterm \<xi>\<^sub>t\<^sub>y' \<xi>\<^sub>t\<^sub>e' \<J>\<^sub>t\<^sub>y \<J> \<L> t"
+  using assms
+proof (induction t)
+  case (Const f \<tau>s ts)
+
+  then have IH': "denotation_preterm \<xi>\<^sub>t\<^sub>y \<xi>\<^sub>t\<^sub>e \<J>\<^sub>t\<^sub>y \<J> \<L> t = denotation_preterm \<xi>\<^sub>t\<^sub>y' \<xi>\<^sub>t\<^sub>e' \<J>\<^sub>t\<^sub>y \<J> \<L> t"
+    if "t \<in> list.set ts" for t
+    using that by simp
+
+  then have "\<J> f (map (denotation_ty \<xi>\<^sub>t\<^sub>y \<J>\<^sub>t\<^sub>y) \<tau>s) (map (denotation_preterm \<xi>\<^sub>t\<^sub>y \<xi>\<^sub>t\<^sub>e \<J>\<^sub>t\<^sub>y \<J> \<L>) ts) =
+    \<J> f (map (denotation_ty \<xi>\<^sub>t\<^sub>y' \<J>\<^sub>t\<^sub>y) \<tau>s) (map (denotation_preterm \<xi>\<^sub>t\<^sub>y' \<xi>\<^sub>t\<^sub>e' \<J>\<^sub>t\<^sub>y \<J> \<L>) ts)"
+    using denotation_ty_of_ground
+    by (metis (mono_tags, lifting) Const.prems(2)
+        UNION_empty_conv(1) list.map_cong0[of \<tau>s] list.map_cong0[of ts]
+        preterm.set_intros(1))
+
+  then show ?case
     by simp
-qed
+next
+  case (Abs \<tau> t)
+  have "\<L> \<xi>\<^sub>t\<^sub>y \<xi>\<^sub>t\<^sub>e (Abs \<tau> t) = \<L> \<xi>\<^sub>t\<^sub>y' \<xi>\<^sub>t\<^sub>e' (Abs \<tau> t)"
+  proof (rule \<L>_depends_only_on_\<xi>_on_vars)
+    show "\<And>\<tau>' x. \<tau>' \<in> type_symbols (Abs \<tau> t) \<Longrightarrow> x \<in> type_vars \<tau>' \<Longrightarrow> \<xi>\<^sub>t\<^sub>y x = \<xi>\<^sub>t\<^sub>y' x"
+      using Abs.prems(2) by blast
+  next
+    show "\<And>x. x \<in> free_vars (Abs \<tau> t) \<Longrightarrow> \<xi>\<^sub>t\<^sub>e x = \<xi>\<^sub>t\<^sub>e' x"
+      by (metis Abs.prems(1) emptyE)
+  qed
 
-lemma not_true_lit_Neg_ident: "\<not> (\<M> \<Turnstile>\<^sub>l (Neg (Upair t t)))"
-  by (simp add: true_lit_Pos_ident)
-
-definition true_cls ::
-  "('\<V>\<^sub>t\<^sub>y, '\<Sigma>\<^sub>t\<^sub>y :: arity, '\<V>, '\<Sigma>, 'd :: domain_universe) model \<Rightarrow>
-    ('\<V>\<^sub>t\<^sub>y, '\<Sigma>\<^sub>t\<^sub>y, '\<V>, '\<Sigma>) atom literal multiset \<Rightarrow> bool"
-  (infix \<open>\<Turnstile>\<^sub>c\<close> 50) where
-  "\<M> \<Turnstile>\<^sub>c C \<longleftrightarrow> (\<exists>L \<in># C. \<M> \<Turnstile>\<^sub>l L)"
-
-locale type_interp_with_bool_and_fun = type_interp \<J>\<^sub>t\<^sub>y
-  for \<J>\<^sub>t\<^sub>y :: "('\<Sigma>\<^sub>t\<^sub>y :: type_signature, 'd :: {domain_universe, zero, one}) type_interp_fun" +
-  assumes
-    zero_neq_one: "(0 :: 'd) \<noteq> 1" and
-    \<J>\<^sub>t\<^sub>y_bool: "\<J>\<^sub>t\<^sub>y bool_tyctr [] = {0, 1}" (* and
-    \<J>\<^sub>t\<^sub>y_fun: "\<And>\<D>\<^sub>1 \<D>\<^sub>2. \<D>\<^sub>1 \<in> \<U> \<Longrightarrow> \<D>\<^sub>2 \<in> \<U> \<Longrightarrow> \<J>\<^sub>t\<^sub>y fun_tyctr [\<D>\<^sub>1, \<D>\<^sub>2] \<subseteq> {}" *)
-
-locale lambda_designation_with_consts = lambda_designation \<J>\<^sub>t\<^sub>y typeof \<L>
-  for \<J>\<^sub>t\<^sub>y :: "('\<Sigma>\<^sub>t\<^sub>y :: type_signature, 'd :: domain_universe) type_interp_fun" and
-    typeof :: "'\<Sigma> :: term_signature \<Rightarrow> ('\<V>\<^sub>t\<^sub>y, '\<Sigma>\<^sub>t\<^sub>y) const_ty" and
-    \<L> :: "('\<V>\<^sub>t\<^sub>y, '\<Sigma>\<^sub>t\<^sub>y, '\<V>, '\<Sigma>, 'd) lambda_designation_fun" +
-  assumes
-    "typeof True_tconst = (Dlist.empty, [], Bool_ty)"
-    "typeof False_tconst = (Dlist.empty, [], Bool_ty)"
-    "typeof Neg_tconst = (Dlist.empty, [], Fun_ty Bool_ty Bool_ty)"
-    "typeof Conj_tconst = (Dlist.empty, [], Fun_ty Bool_ty (Fun_ty Bool_ty Bool_ty))"
-    "typeof Disj_tconst = (Dlist.empty, [], Fun_ty Bool_ty (Fun_ty Bool_ty Bool_ty))"
-    "typeof Imp_tconst = (Dlist.empty, [], Fun_ty Bool_ty (Fun_ty Bool_ty Bool_ty))"
-    "\<exists>(x :: '\<V>\<^sub>t\<^sub>y). typeof Eq_tconst = (Dlist [x], [], Fun_ty (Tyvar_ty x) (Fun_ty (Tyvar_ty x) Bool_ty))"
-    "\<exists>(x :: '\<V>\<^sub>t\<^sub>y). typeof Neq_tconst = (Dlist[x], [], Fun_ty (Tyvar_ty x) (Fun_ty (Tyvar_ty x) Bool_ty))"
+  then show ?case
+    by simp
+qed simp_all
 
 
-datatype mytypes = MyBool | MyInt | MyList | MyFun
+subsection \<open>Rest\<close>
 
-instantiation mytypes :: arity
+locale proper_interp = interp +
+  assumes "app (\<L> \<xi>\<^sub>t\<^sub>y \<xi> (Abs \<tau> t)) a = \<L> \<xi>\<^sub>t\<^sub>y (\<xi>(x := a)) (subst_bound 0 (Free x) t)"
+
+print_locale interp
+
+declare [[typedef_overloaded]]
+record ('\<V>\<^sub>t\<^sub>y, '\<Sigma>\<^sub>t\<^sub>y :: arity, '\<V>, '\<Sigma>) interp =
+  \<U> :: "V set"
+  \<C> :: "'\<Sigma> \<Rightarrow> '\<V>\<^sub>t\<^sub>y dlist \<times> ('\<V>\<^sub>t\<^sub>y, '\<Sigma>\<^sub>t\<^sub>y) ty list \<times> ('\<V>\<^sub>t\<^sub>y, '\<Sigma>\<^sub>t\<^sub>y) ty"
+  \<J>\<^sub>t\<^sub>y :: "'\<Sigma>\<^sub>t\<^sub>y \<Rightarrow> V list \<Rightarrow> V"
+  \<J> :: "'\<Sigma> \<Rightarrow> V list \<Rightarrow> V list \<Rightarrow> V"
+  \<L> :: "('\<V>\<^sub>t\<^sub>y \<Rightarrow> V) \<Rightarrow> ('\<V> \<Rightarrow> V) \<Rightarrow> (('\<V>\<^sub>t\<^sub>y, '\<Sigma>\<^sub>t\<^sub>y) ty, '\<Sigma>, '\<V>) preterm \<Rightarrow> V"
+
+type_synonym ('\<V>\<^sub>t\<^sub>y, '\<Sigma>\<^sub>t\<^sub>y, '\<V>, '\<Sigma>) atom = "(('\<V>\<^sub>t\<^sub>y, '\<Sigma>\<^sub>t\<^sub>y) ty, '\<Sigma>, '\<V>) preterm uprod"
+datatype 'a literal =
+  is_pos: Pos (atom: 'a) |
+  is_neg: Neg (atom: 'a)
+
+instantiation literal :: (type) uminus
 begin
 
-definition arity_mytypes :: "mytypes \<Rightarrow> nat" where
-  "arity_mytypes \<tau> \<equiv>
-    (case \<tau> of
-      MyBool \<Rightarrow> 0 |
-      MyInt \<Rightarrow> 0 |
-      MyList \<Rightarrow> 1 |
-      MyFun \<Rightarrow> 2)"
+primrec uminus_literal :: "'a literal \<Rightarrow> 'a literal" where
+  "uminus (Pos A) = Neg A" |
+  "uminus (Neg A) = Pos A"
 
 instance ..
 
 end
 
-lemma arity_mytypes_simps[simp]:
-  "arity MyBool = 0"
-  "arity MyInt = 0"
-  "arity MyList = 1"
-  "arity MyFun = 2"
-  by (simp_all add: arity_mytypes_def)
+fun true_lit ::
+  "('\<V>\<^sub>t\<^sub>y, '\<Sigma>\<^sub>t\<^sub>y :: arity, '\<V>, '\<Sigma>) interp \<times> ('\<V>\<^sub>t\<^sub>y \<Rightarrow> V) \<times> ('\<V> \<Rightarrow> V) \<Rightarrow>
+    ('\<V>\<^sub>t\<^sub>y, '\<Sigma>\<^sub>t\<^sub>y, '\<V>, '\<Sigma>) atom literal \<Rightarrow> bool"
+  (infix \<open>\<Turnstile>\<^sub>l\<close> 50) where
+  "(\<I>, \<xi>\<^sub>t\<^sub>y, \<xi>\<^sub>t\<^sub>e) \<Turnstile>\<^sub>l (Pos A) \<longleftrightarrow> (case_uprod (Abs_commute (=))
+    (map_uprod (denotation_preterm \<xi>\<^sub>t\<^sub>y \<xi>\<^sub>t\<^sub>e (interp.\<J>\<^sub>t\<^sub>y \<I>) (interp.\<J> \<I>) (interp.\<L> \<I>)) A))" |
+  "(\<I>, \<xi>\<^sub>t\<^sub>y, \<xi>\<^sub>t\<^sub>e) \<Turnstile>\<^sub>l (Neg A) \<longleftrightarrow> (case_uprod (Abs_commute (\<noteq>))
+    (map_uprod (denotation_preterm \<xi>\<^sub>t\<^sub>y \<xi>\<^sub>t\<^sub>e (interp.\<J>\<^sub>t\<^sub>y \<I>) (interp.\<J> \<I>) (interp.\<L> \<I>)) A))"
 
-lemma "wf_prety (PretyCtr MyList [PretyCtr MyInt []])"
-proof (intro wf_prety.PretyCtr ballI)
-  show "length [PretyCtr MyInt []] = arity MyList"
-    by (simp add: arity_mytypes_def)
-next
-  show "\<And>\<tau>. \<tau> \<in> set [PretyCtr MyInt []] \<Longrightarrow> wf_prety \<tau>"
-    by (auto simp add: arity_mytypes_def intro: wf_prety.intros)
-qed
+lemma true_lit_iff_not_true_uminus_lit[simp]: "\<not> (\<I>\<xi> \<Turnstile>\<^sub>l L) \<longleftrightarrow> \<I>\<xi> \<Turnstile>\<^sub>l (-L)"
+  by (cases \<I>\<xi>, cases L) simp_all
 
-lemma "\<not> wf_prety (PretyCtr MyList [])"
-  using wf_prety.cases by fastforce
+lemma true_lit_Pos_ident: "\<I>\<xi> \<Turnstile>\<^sub>l (Pos (Upair t t))"
+  by (cases \<I>\<xi>) simp
 
-instantiation mytypes :: type_signature
-begin
+lemma not_true_lit_Neg_ident: "\<not> (\<I>\<xi> \<Turnstile>\<^sub>l (Neg (Upair t t)))"
+  by (cases \<I>\<xi>) simp
 
-definition "bool_tyctr_mytypes \<equiv> MyBool"
-definition "fun_tyctr_mytypes \<equiv> MyFun"
+definition true_cls ::
+  "('\<V>\<^sub>t\<^sub>y, '\<Sigma>\<^sub>t\<^sub>y :: arity, '\<V>, '\<Sigma>) interp \<times> ('\<V>\<^sub>t\<^sub>y \<Rightarrow> V) \<times> ('\<V> \<Rightarrow> V) \<Rightarrow>
+    ('\<V>\<^sub>t\<^sub>y, '\<Sigma>\<^sub>t\<^sub>y, '\<V>, '\<Sigma>) atom literal multiset \<Rightarrow> bool"
+  (infix \<open>\<Turnstile>\<^sub>c\<close> 50) where
+  "\<I>\<xi> \<Turnstile>\<^sub>c C \<longleftrightarrow> (\<exists>L \<in># C. \<I>\<xi> \<Turnstile>\<^sub>l L)"
 
-instance
-  by standard (simp_all add: bool_tyctr_mytypes_def fun_tyctr_mytypes_def)
+print_locale proper_interp
 
-end
-
-datatype mydomain = Dint int | Dbool bool | Dlist "mydomain list"
-
-fun mytypeinterp where
-  "mytypeinterp MyInt \<D>s = (if \<D>s = [] then Some {Dint n | n :: int. True} else None)" |
-  "mytypeinterp MyBool \<D>s = (if \<D>s = [] then Some {Dbool b | b :: bool. True} else None)" |
-  "mytypeinterp MyList \<D>s = (case \<D>s of [\<D>] \<Rightarrow> Some {Dlist ds | ds :: mydomain list. set ds \<subseteq> \<D>} | _ \<Rightarrow> None)"
-
-inductive_set myuniverse where
-  "{Dint n | n :: int. True} \<in> myuniverse" |
-  "{Dbool b | b :: bool. True} \<in> myuniverse" |
-  "\<D> \<in> myuniverse \<Longrightarrow> {Dlist ds | ds :: mydomain list. set ds \<subseteq> \<D>} \<in> myuniverse"
-
-interpretation semantics where
-  \<U> = "myuniverse" and
-  \<J>\<^sub>t\<^sub>y = "mytypeinterp"
-proof unfold_locales
-  show "{} \<notin> myuniverse"
-    by (metis (mono_tags, lifting)
-        empty_Collect_eq empty_subsetI
-        list.set(1) myuniverse.simps)
-next
-  fix \<kappa> \<D>s
-  show "(arity \<kappa> = length \<D>s) = (mytypeinterp \<kappa> \<D>s \<noteq> None)"
-  proof (cases \<kappa>)
-    case MyBool
-    then show ?thesis
-      by simp
-  next
-    case MyInt
-    then show ?thesis
-      by simp
-  next
-    case MyList
-    then show ?thesis
-    proof (cases "\<exists>\<D>. \<D>s = [\<D>]")
-      case True
-      then show ?thesis
-        using MyList by auto
-    next
-      case False
-      then show ?thesis
-        unfolding MyList arity_mytypes_simps
-        by (metis (no_types, lifting) One_nat_def Suc_le_eq
-            impossible_Cons length_Cons length_greater_0_conv
-            list.simps(4,5) list.size(3) mytypeinterp.simps(3)
-            neq_Nil_conv)
-    qed
-  next
-    case MyFun
-    then show ?thesis
-      sorry
-  qed
-qed
+definition true_clss ::
+  "('\<V>\<^sub>t\<^sub>y, '\<Sigma>\<^sub>t\<^sub>y :: type_signature, '\<V>, '\<Sigma>) interp \<Rightarrow>
+    ('\<V>\<^sub>t\<^sub>y, '\<Sigma>\<^sub>t\<^sub>y, '\<V>, '\<Sigma>) atom literal multiset set \<Rightarrow> bool"
+  (infix \<open>\<Turnstile>\<^sub>c\<^sub>s\<close> 50) where
+  "\<I> \<Turnstile>\<^sub>c\<^sub>s N \<longleftrightarrow>
+    proper_interp (interp.\<U> \<I>) (interp.\<J>\<^sub>t\<^sub>y \<I>) (interp.\<C> \<I>) (interp.\<J> \<I>) (interp.\<L> \<I>) \<and>
+    (\<forall>\<xi>\<^sub>t\<^sub>y \<xi>\<^sub>t\<^sub>e. \<forall>C \<in> N. (\<I>, \<xi>\<^sub>t\<^sub>y, \<xi>\<^sub>t\<^sub>e) \<Turnstile>\<^sub>c C)"
 
 end
